complete ReprBetree interface

Splinter/Betree/ReprBetree.i.dfy
@@ -5,6 +5,7 @@ include "LinkedBetree.i.dfy"
 include "../../lib/Buckets/BoundedPivotsLib.i.dfy"
 include "../Journal/GenericDisk.i.dfy"
 include "Domain.i.dfy"
+include "SplitRequest.i.dfy"
 
 module ReprBetree
 {
@@ -18,6 +19,7 @@ module ReprBetree
   import opened MemtableMod
   import opened MsgHistoryMod
   import opened Sequences
+  import opened SplitRequestMod
   import LinkedBetreeMod
 
   type Pointer = GenericDisk.Pointer
@@ -25,24 +27,35 @@ module ReprBetree
 
   type StampedBetree = LinkedBetreeMod.StampedBetree
   type LinkedBetree = LinkedBetreeMod.LinkedBetree
-  type Step = LinkedBetreeMod.Step
+  type Path = LinkedBetreeMod.Path
+  type PathAddrs = LinkedBetreeMod.PathAddrs
+  type SplitAddrs = LinkedBetreeMod.SplitAddrs
   type QueryReceipt = LinkedBetreeMod.QueryReceipt
+
+  datatype GCBetree = GCBetree(
+    reserved: seq<Address>,
+    stranded: set<Address>,
+    stamped: StampedBetree
+  )
   
   // Copied from linkedJournal, except for InternalLabel
   datatype TransitionLabel =
       QueryLabel(endLsn: LSN, key: Key, value: Value)
     | PutLabel(puts: MsgHistory)
     | QueryEndLsnLabel(endLsn: LSN)
-    | FreezeAsLabel(linkedBetree: StampedBetree)
-    | InternalLabel(addrs: seq<Address>, freedAddrs: set<Address>) 
+    | FreezeAsLabel(gcBetree: GCBetree)
+    // Internal-x labels refine to no-ops at the abstract spec
+    | InternalMapGCLabel(allocations: seq<Address>, freed: set<Address>)
+    | InternalLabel() 
   {
     function I() : LinkedBetreeMod.TransitionLabel {
       match this {
         case QueryLabel(endLsn, key, value) => LinkedBetreeMod.QueryLabel(endLsn, key, value)
         case PutLabel(puts) => LinkedBetreeMod.PutLabel(puts)
         case QueryEndLsnLabel(endLsn) => LinkedBetreeMod.QueryEndLsnLabel(endLsn)
-        case FreezeAsLabel(linkedBetree) => LinkedBetreeMod.FreezeAsLabel(linkedBetree)
-        case InternalLabel(addrs, _) => LinkedBetreeMod.InternalLabel(addrs)
+        case FreezeAsLabel(gcBetree) => LinkedBetreeMod.FreezeAsLabel(gcBetree.stamped)
+        case InternalMapGCLabel(_, _) => LinkedBetreeMod.InternalLabel()
+        case InternalLabel() => LinkedBetreeMod.InternalLabel()
       }
     }
   }
@@ -50,7 +63,9 @@ module ReprBetree
   datatype Variables = Variables(
     betree: LinkedBetreeMod.Variables,
     // maps each in-repr node n to the representation of the subtree with that node as root
-    repr: set<Address>)
+    repr: set<Address>,
+    reserved: seq<Address>,
+    stranded: set<Address>)
   {
     predicate WF() {
       betree.WF()
@@ -84,6 +99,9 @@ module ReprBetree
   predicate FreezeAs(v: Variables, v': Variables, lbl: TransitionLabel)
   {
     && LinkedBetreeMod.FreezeAs(v.betree, v'.betree, lbl.I())
+    // we only remember a subset of our reserved and stranded set as we freeze
+    && IsPrefix(lbl.gcBetree.reserved, v.reserved)
+    && lbl.gcBetree.stranded <= v.stranded 
     && v' == v.(
       betree := v'.betree
     )
@@ -91,7 +109,7 @@ module ReprBetree
 
   predicate InternalGrow(v: Variables, v': Variables, lbl: TransitionLabel, step: Step)
   {
-    && LinkedBetreeMod.InternalGrow(v.betree, v'.betree, lbl.I(), step)
+    && LinkedBetreeMod.InternalGrow(v.betree, v'.betree, lbl.I(), step.I())
     && v' == v.(
       betree := v'.betree,
       repr := v.repr + {step.newRootAddr}
@@ -122,13 +140,83 @@ module ReprBetree
     false
   }
 
-  predicate Init(v: Variables, stampedBetree: StampedBetree)
+  predicate InternalMapReserve(v: Variables, v': Variables, lbl: TransitionLabel)
+  {
+    // Enabling conditions
+    && lbl.InternalMapGCLabel?
+    && v.WF()
+    && 0 < |lbl.allocations|
+    && lbl.freed == {}
+    // State transition
+    && v' == v.(
+      reserved := v.reserved + lbl.allocations
+    )
+  }
+
+  predicate InternalMapFree(v: Variables, v': Variables, lbl: TransitionLabel)
+  {
+    // Enabling conditions
+    && lbl.InternalMapGCLabel?
+    && v.WF()
+    && lbl.allocations == []
+    && lbl.freed <= v.stranded
+    && 0 < |lbl.freed|
+    // State transition
+    && v' == v.(
+      stranded := v.stranded - lbl.freed
+    )
+  }
+
+  predicate InternalNoOp(v: Variables, v': Variables, lbl: TransitionLabel)
+  {
+    && lbl.InternalLabel?
+    && v.WF()
+    && v' == v
+  }
+
+  predicate Init(v: Variables, gcBetree: GCBetree)
   {
     && v.betree.linked.Acyclic()
     && v == Variables(
-      LinkedBetreeMod.Variables(EmptyMemtable(stampedBetree.seqEnd), stampedBetree.value),
-      v.betree.linked.ReachableAddrs()
+      LinkedBetreeMod.Variables(EmptyMemtable(gcBetree.stamped.seqEnd), gcBetree.stamped.value),
+      v.betree.linked.ReachableAddrs(),
+      gcBetree.reserved,
+      gcBetree.stranded
     )
+  }
+
+  datatype Step =
+      QueryStep(receipt: QueryReceipt)
+    | PutStep()
+    | QueryEndLsnStep()
+    | FreezeAsStep()
+    | InternalGrowStep(newRootAddr: Address)
+    | InternalSplitStep(path: Path, request: SplitRequest, newAddrs: SplitAddrs, pathAddrs: PathAddrs)
+    | InternalFlushMemtableStep(newRootAddr: Address)
+    | InternalFlushStep(path: Path, childIdx: nat, targetAddr: Address, targetChildAddr: Address, pathAddrs: PathAddrs)
+    | InternalCompactStep(path: Path, compactedBuffers: BufferStack, targetAddr: Address, pathAddrs: PathAddrs)
+    | InternalMapReserveStep()    // reserve more addresses from the global allocator
+    | InternalMapFreeStep()       // free some stranded addresses
+    | InternalNoOpStep()
+  {
+    function I() : LinkedBetreeMod.Step {
+      match this {
+        case QueryStep(receipt) => LinkedBetreeMod.QueryStep(receipt)
+        case PutStep() => LinkedBetreeMod.PutStep()
+        case QueryEndLsnStep() => LinkedBetreeMod.QueryEndLsnStep()
+        case FreezeAsStep() => LinkedBetreeMod.FreezeAsStep()
+        case InternalGrowStep(newRootAddr) => LinkedBetreeMod.InternalGrowStep(newRootAddr)
+        case InternalSplitStep(path, reqeust, newAddrs, pathAddrs) => 
+              LinkedBetreeMod.InternalSplitStep(path, reqeust, newAddrs, pathAddrs)
+        case InternalFlushStep(path, childIdx, targetAddr, targetChildAddr, pathAddrs) => 
+              LinkedBetreeMod.InternalFlushStep(path, childIdx, targetAddr, targetChildAddr, pathAddrs)
+        case InternalFlushMemtableStep(newRootAddr) => LinkedBetreeMod.InternalFlushMemtableStep(newRootAddr)
+        case InternalCompactStep(path, compactedBuffers, targetAddr, pathAddrs) => LinkedBetreeMod.InternalCompactStep(path, compactedBuffers, targetAddr, pathAddrs)
+        case InternalMapReserveStep() => LinkedBetreeMod.InternalNoOpStep()
+        case InternalMapFreeStep() => LinkedBetreeMod.InternalNoOpStep()
+        case InternalNoOpStep() => LinkedBetreeMod.InternalNoOpStep()
+      }
+    }
   }
 
   predicate NextStep(v: Variables, v': Variables, lbl: TransitionLabel, step: Step)
@@ -143,6 +231,9 @@ module ReprBetree
       case InternalFlushStep(_, _, _, _, _) => InternalFlush(v, v', lbl, step)
       case InternalFlushMemtableStep(_) => InternalFlushMemtable(v, v', lbl, step)
       case InternalCompactStep(_, _, _, _) => InternalCompact(v, v', lbl, step)
+      case InternalMapReserveStep() => InternalMapReserve(v, v', lbl)
+      case InternalMapFreeStep() => InternalMapFree(v, v', lbl)
+      case InternalNoOpStep() => InternalNoOp(v, v', lbl)
     }
   }
 
